sat2.dfy
@@ -1,0 +1,67 @@
+include "sat.dfy"
+
+datatype Expression2 =
+    Constant2(bool) |
+    Var2(Variable, bool) |
+    And2(Expression2, Expression2) |
+    Or2(Expression2,Expression2)
+{
+    static function from_Expression(e: Expression) : (ee: Expression2)
+        requires e.Valid()
+        requires e.no_implies()
+        requires e.no_equivalent()
+        requires e.no_not()
+        ensures ee.Valid()
+        ensures forall vs : map<Variable, bool> :: true ==>
+            e.eval(vs) == ee.eval(vs)
+    {
+        match e {
+            case Constant(b) => Constant2(b)
+            case Var(v, i) => Var2(v, i)
+            case And(a,b) => And2(from_Expression(a),from_Expression(b))
+            case Or(a,b) => Or2(from_Expression(a),from_Expression(b))
+            case Not(_) | Implies(_,_) | Equivalent(_,_) => 
+                assert false; Constant2(false)
+        }
+    }
+
+    function children() : (cs: set<Expression2>)
+    {
+        match this {
+            case Constant2(b) => {}
+            case Var2(v, _) => {}
+            case And2(a,b) => {a, b}
+            case Or2(a,b) => {a, b}
+        }
+    }
+    
+    ghost function height() : (h: int)
+        ensures h >= 1
+    {
+        match this {
+            case Constant2(b) => 1
+            case Var2(v, _) => 1
+            case And2(a,b) => 1 + max(a.height(), b.height())
+            case Or2(a,b) => 1 + max(a.height(), b.height())
+        }
+    }
+
+    ghost predicate Valid()
+    {
+        forall i :: i in children() ==> i.Valid() && i.height() < this.height()
+    }
+
+    function eval(vs: map<Variable,bool>) : (b: bool)
+        requires this.Valid()
+        decreases this
+    {
+        match this {
+            case Constant2(b) => b
+            case Var2(v, inverted) =>
+                var val := if v in vs then vs[v] else false;
+                if inverted then val else !val
+            case And2(a,b) => a.eval(vs) && b.eval(vs)
+            case Or2(a,b) => a.eval(vs) || b.eval(vs)
+        }
+    }
+}
